theories/input_lang_callcc/lang.v
@@ -1,0 +1,563 @@
+From stdpp Require Export strings.
+From gitrees Require Export prelude.
+From Equations Require Import Equations.
+Require Import List.
+Import ListNotations.
+
+Require Import Binding.Lib Binding.Set Binding.Auto Binding.Env.
+
+Inductive nat_op := Add | Sub | Mult.
+
+Inductive expr {X : Set} :=
+(* Values *)
+| Val (v : val) : expr
+(* Base lambda calculus *)
+| App (e₁ : expr) (e₂ : expr) : expr
+(* Base types and their operations *)
+| NatOp (op : nat_op) (e₁ : expr) (e₂ : expr) : expr
+| If (e₁ : expr) (e₂ : expr) (e₃ : expr) : expr
+(* The effects *)
+| Input : expr
+| Output (e : expr) : expr
+| Callcc (e : @expr (inc X)) : expr
+| Throw (e₁ : expr) (e₂ : expr) : expr
+with val {X : Set} :=
+| VarV (x : X) : val
+| LitV (n : nat) : val
+| RecV (e : @expr (inc (inc X))) : val
+| ContV (K : ectx) : val
+with ectx {X : Set} :=
+| EmptyK : ectx
+| OutputK (K : ectx) : ectx
+| IfK (K : ectx) (e₁ : expr) (e₂ : expr) : ectx
+| AppLK (e : expr) (K : ectx) : ectx
+| AppRK (K : ectx) (v : val) : ectx
+| NatOpLK (op : nat_op) (e : expr) (K : ectx) : ectx
+| NatOpRK (op : nat_op) (K : ectx) (v : val) : ectx
+| ThrowLK (K : ectx) (e : expr) : ectx
+| ThrowRK (v : val) (K : ectx) : ectx.
+
+Notation of_val := Val (only parsing).
+
+Arguments val X%bind : clear implicits.
+Arguments expr X%bind : clear implicits.
+Arguments ectx X%bind : clear implicits.
+
+Declare Scope syn_scope.
+Declare Scope ectx_scope.
+Delimit Scope syn_scope with syn.
+Delimit Scope ectx_scope with ectx.
+
+Coercion Val : val >-> expr.
+Coercion App : expr >-> Funclass.
+Coercion AppLK : expr >-> Funclass.
+Coercion AppRK : ectx >-> Funclass.
+
+Notation "+" := (Add) : syn_scope.
+Notation "-" := (Sub) : syn_scope.
+Notation "×" := (Mult) : syn_scope.
+Notation "'⟨' e₁ op e₂ '⟩'" := (NatOp op e₁ e₂) (at level 45, right associativity) : syn_scope.
+Notation "'if' e₁ 'then' e₂ 'else' e₃" := (If e₁ e₂ e₃) : syn_scope.
+Notation "'#' n" := (LitV n) (at level 60) : syn_scope.
+Notation "'input'" := (Input) : syn_scope.
+Notation "'output' e" := (Output e) (at level 60) : syn_scope.
+Notation "'rec' e" := (RecV e) (at level 60) : syn_scope.
+Notation "'throw' e₁ e₂" := (Throw e₁ e₂) (at level 60) : syn_scope.
+Notation "'cont' K" := (ContV K) (at level 60) : syn_scope.
+
+Notation "□" := (EmptyK) : ectx_scope.
+Notation "'⟨' e₁ op K '⟩ᵣ'" := (NatOpLK op e₁ K) (at level 45, right associativity) : ectx_scope.
+Notation "'⟨' K op v₂ '⟩ₗ'" := (NatOpRK op K v₂) (at level 45, right associativity) : ectx_scope.
+Notation "'if' K 'then' e₂ 'else' e₃" := (IfK K e₂ e₃) : ectx_scope.
+Notation "'output' K" := (OutputK K) (at level 60) : ectx_scope.
+Notation "'throwₗ' K e₂" := (ThrowLK K e₂) (at level 60) : ectx_scope.
+Notation "'throwᵣ' e₁ K" := (ThrowRK e₁ K) (at level 60) : ectx_scope.
+
+Definition to_val {S} (e : expr S) : option (val S) :=
+  match e with
+  | Val v => Some v
+  | _ => None
+  end.
+
+Definition do_natop (op : nat_op) (x y : nat) : nat :=
+  match op with
+  | Add => plus x y
+  | Sub => minus x y
+  | Mult => mult x y
+  end.
+
+Definition nat_op_interp {S} (n : nat_op) (x y : val S) : option (val S) :=
+  match x, y with
+  | LitV x, LitV y => Some $ LitV $ do_natop n x y
+  | _,_ => None
+  end.
+
+Fixpoint fill {X : Set} (K : ectx X) (e : expr X) : expr X :=
+  match K with
+  | EmptyK => e
+  | OutputK K => Output (fill K e)
+  | IfK K e₁ e₂ => If (fill K e) e₁ e₂
+  | AppLK e' K => App e' (fill K e)
+  | AppRK K v => App (fill K e) (Val v)
+  | NatOpLK op e' K => NatOp op e' (fill K e)
+  | NatOpRK op K v => NatOp op (fill K e) (Val v)
+  | ThrowLK K e' => Throw (fill K e) e'
+  | ThrowRK v K => Throw (Val v) (fill K e)
+  end.
+
+Notation "K '[' e ']'" := (fill K e) (at level 60) : syn_scope.
+
+Local Open Scope bind_scope.
+
+Fixpoint emap {A B : Set} (f : A [→] B) (e : expr A) : expr B :=
+  match e with
+  | Val v => Val (vmap f v)
+  | App e₁ e₂ => App (emap f e₁) (emap f e₂)
+  | NatOp o e₁ e₂ => NatOp o (emap f e₁) (emap f e₂)
+  | If e₁ e₂ e₃ => If (emap f e₁) (emap f e₂) (emap f e₃)
+  | Input => Input
+  | Output e => Output (emap f e)
+  | Callcc e => Callcc (emap (f ↑) e)
+  | Throw e₁ e₂ => Throw (emap f e₁) (emap f e₂)
+  end
+with vmap {A B : Set} (f : A [→] B) (v : val A) : val B :=
+       match v with
+       | VarV x => VarV (f x)
+       | LitV n => LitV n
+       | RecV e => RecV (emap ((f ↑) ↑) e)
+       | ContV K => ContV (kmap f K)
+       end
+with kmap {A B : Set} (f : A [→] B) (K : ectx A) : ectx B :=
+       match K with
+       | EmptyK => EmptyK
+       | OutputK K => OutputK (kmap f K)
+       | IfK K e₁ e₂ => IfK (kmap f K) (emap f e₁) (emap f e₂)
+       | AppLK e K => AppLK (emap f e) (kmap f K)
+       | AppRK K v => AppRK (kmap f K) (vmap f v)
+       | NatOpLK op e K => NatOpLK op (emap f e) (kmap f K)
+       | NatOpRK op K v => NatOpRK op (kmap f K) (vmap f v)
+       | ThrowLK K e => ThrowLK (kmap f K) (emap f e)
+       | ThrowRK v K => ThrowRK (vmap f v) (kmap f K)
+       end.
+#[export] Instance FMap_expr : FunctorCore expr := @emap.
+#[export] Instance FMap_val  : FunctorCore val := @vmap.
+#[export] Instance FMap_ectx  : FunctorCore ectx := @kmap.
+
+Lemma fill_emap {X Y : Set} (f : X [→] Y) (K : ectx X) (e : expr X)
+  : fmap f (fill K e) = fill (fmap f K) (fmap f e).
+Proof.
+  revert f.
+  induction K as [| ?? IH
+                 | ?? IH
+                 | ??? IH
+                 | ?? IH
+                 | ???? IH
+                 | ??? IH
+                 | ?? IH
+                 | ??? IH];
+    intros f; term_simpl; first done; rewrite IH; reflexivity.
+Qed.
+
+#[export] Instance SPC_val : SetPureCore val := @VarV.
+
+Fixpoint ebind {A B : Set} (f : A [⇒] B) (e : expr A) : expr B :=
+  match e with
+  | Val v => Val (vbind f v)
+  | App e₁ e₂ => App (ebind f e₁) (ebind f e₂)
+  | NatOp o e₁ e₂ => NatOp o (ebind f e₁) (ebind f e₂)
+  | If e₁ e₂ e₃ => If (ebind f e₁) (ebind f e₂) (ebind f e₃)
+  | Input => Input
+  | Output e => Output (ebind f e)
+  | Callcc e => Callcc (ebind (f ↑) e)
+  | Throw e₁ e₂ => Throw (ebind f e₁) (ebind f e₂)
+  end
+with vbind {A B : Set} (f : A [⇒] B) (v : val A) : val B :=
+       match v with
+       | VarV x => f x
+       | LitV n => LitV n
+       | RecV e => RecV (ebind ((f ↑) ↑) e)
+       | ContV K => ContV (kbind f K)
+       end
+with kbind {A B : Set} (f : A [⇒] B) (K : ectx A) : ectx B :=
+       match K with
+       | EmptyK => EmptyK
+       | OutputK K => OutputK (kbind f K)
+       | IfK K e₁ e₂ => IfK (kbind f K) (ebind f e₁) (ebind f e₂)
+       | AppLK e K => AppLK (ebind f e) (kbind f K)
+       | AppRK K v => AppRK (kbind f K) (vbind f v)
+       | NatOpLK op e K => NatOpLK op (ebind f e) (kbind f K)
+       | NatOpRK op K v => NatOpRK op (kbind f K) (vbind f v)
+       | ThrowLK K e => ThrowLK (kbind f K) (ebind f e)
+       | ThrowRK v K => ThrowRK (vbind f v) (kbind f K)
+       end.
+
+#[export] Instance BindCore_expr : BindCore expr := @ebind.
+#[export] Instance BindCore_val  : BindCore val := @vbind.
+#[export] Instance BindCore_ectx  : BindCore ectx := @kbind.
+
+#[export] Instance IP_typ : SetPure val.
+Proof.
+  split; intros; reflexivity.
+Qed.
+
+Fixpoint vmap_id X (δ : X [→] X) (v : val X) : δ ≡ ı → fmap δ v = v
+with emap_id X (δ : X [→] X) (e : expr X) : δ ≡ ı → fmap δ e = e
+with kmap_id X (δ : X [→] X) (e : ectx X) : δ ≡ ı → fmap δ e = e.
+Proof.
+  - auto_map_id.
+  - auto_map_id.
+  - auto_map_id.
+Qed.
+
+Fixpoint vmap_comp (A B C : Set) (f : B [→] C) (g : A [→] B) h (v : val A) :
+  f ∘ g ≡ h → fmap f (fmap g v) = fmap h v
+with emap_comp (A B C : Set) (f : B [→] C) (g : A [→] B) h (e : expr A) :
+  f ∘ g ≡ h → fmap f (fmap g e) = fmap h e
+with kmap_comp (A B C : Set) (f : B [→] C) (g : A [→] B) h (e : ectx A) :
+  f ∘ g ≡ h → fmap f (fmap g e) = fmap h e.
+Proof.
+  - auto_map_comp.
+  - auto_map_comp.
+  - auto_map_comp.
+Qed.
+
+#[export] Instance Functor_val : Functor val.
+Proof.
+  split; [exact vmap_id | exact vmap_comp].
+Qed.
+#[export] Instance Functor_expr : Functor expr.
+Proof.
+  split; [exact emap_id | exact emap_comp].
+Qed.
+#[export] Instance Functor_ectx : Functor ectx.
+Proof.
+  split; [exact kmap_id | exact kmap_comp].
+Qed.
+
+Fixpoint vmap_vbind_pure (A B : Set) (f : A [→] B) (g : A [⇒] B) (v : val A) :
+  f ̂ ≡ g → fmap f v = bind g v
+with emap_ebind_pure (A B : Set) (f : A [→] B) (g : A [⇒] B) (e : expr A) :
+  f ̂ ≡ g → fmap f e = bind g e
+with kmap_kbind_pure (A B : Set) (f : A [→] B) (g : A [⇒] B) (e : ectx A) :
+  f ̂ ≡ g → fmap f e = bind g e.
+Proof.
+  - auto_map_bind_pure.
+    erewrite emap_ebind_pure; [reflexivity |].
+    intros [| [| x]]; term_simpl; [reflexivity | reflexivity |].
+    rewrite <-(EQ x).
+    reflexivity.
+  - auto_map_bind_pure.
+  - auto_map_bind_pure.
+Qed.
+
+#[export] Instance BindMapPure_val : BindMapPure val.
+Proof.
+  split; intros; now apply vmap_vbind_pure.
+Qed.
+#[export] Instance BindMapPure_expr : BindMapPure expr.
+Proof.
+  split; intros; now apply emap_ebind_pure.
+Qed.
+#[export] Instance BindMapPure_ectx : BindMapPure ectx.
+Proof.
+  split; intros; now apply kmap_kbind_pure.
+Qed.
+
+Fixpoint vmap_vbind_comm (A B₁ B₂ C : Set) (f₁ : B₁ [→] C) (f₂ : A [→] B₂)
+  (g₁ : A [⇒] B₁) (g₂ : B₂ [⇒] C) (v : val A) :
+  g₂ ∘ f₂ ̂ ≡ f₁ ̂ ∘ g₁ → bind g₂ (fmap f₂ v) = fmap f₁ (bind g₁ v)
+with emap_ebind_comm (A B₁ B₂ C : Set) (f₁ : B₁ [→] C) (f₂ : A [→] B₂)
+       (g₁ : A [⇒] B₁) (g₂ : B₂ [⇒] C) (e : expr A) :
+  g₂ ∘ f₂ ̂ ≡ f₁ ̂ ∘ g₁ → bind g₂ (fmap f₂ e) = fmap f₁ (bind g₁ e)
+with kmap_kbind_comm (A B₁ B₂ C : Set) (f₁ : B₁ [→] C) (f₂ : A [→] B₂)
+       (g₁ : A [⇒] B₁) (g₂ : B₂ [⇒] C) (e : ectx A) :
+  g₂ ∘ f₂ ̂ ≡ f₁ ̂ ∘ g₁ → bind g₂ (fmap f₂ e) = fmap f₁ (bind g₁ e).
+Proof.
+  - auto_map_bind_comm.
+    erewrite emap_ebind_comm; [reflexivity |].
+    erewrite lift_comm; [reflexivity |].
+    erewrite lift_comm; [reflexivity | assumption].
+  - auto_map_bind_comm.
+  - auto_map_bind_comm.
+Qed.
+
+#[export] Instance BindMapComm_val : BindMapComm val.
+Proof.
+  split; intros; now apply vmap_vbind_comm.
+Qed.
+#[export] Instance BindMapComm_expr : BindMapComm expr.
+Proof.
+  split; intros; now apply emap_ebind_comm.
+Qed.
+#[export] Instance BindMapComm_ectx : BindMapComm ectx.
+Proof.
+  split; intros; now apply kmap_kbind_comm.
+Qed.
+
+Fixpoint vbind_id (A : Set) (f : A [⇒] A) (v : val A) :
+  f ≡ ı → bind f v = v
+with ebind_id  (A : Set) (f : A [⇒] A) (e : expr A) :
+  f ≡ ı → bind f e = e
+with kbind_id  (A : Set) (f : A [⇒] A) (e : ectx A) :
+  f ≡ ı → bind f e = e.
+Proof.
+  - auto_bind_id.
+    rewrite ebind_id; [reflexivity |].
+    apply lift_id, lift_id; assumption.
+  - auto_bind_id.
+  - auto_bind_id.
+Qed.
+
+Fixpoint vbind_comp (A B C : Set) (f : B [⇒] C) (g : A [⇒] B) h (v : val A) :
+  f ∘ g ≡ h → bind f (bind g v) = bind h v
+with ebind_comp (A B C : Set) (f : B [⇒] C) (g : A [⇒] B) h (e : expr A) :
+  f ∘ g ≡ h → bind f (bind g e) = bind h e
+with kbind_comp (A B C : Set) (f : B [⇒] C) (g : A [⇒] B) h (e : ectx A) :
+  f ∘ g ≡ h → bind f (bind g e) = bind h e.
+Proof.
+  - auto_bind_comp.
+    erewrite ebind_comp; [reflexivity |].
+    erewrite lift_comp; [reflexivity |].
+    erewrite lift_comp; [reflexivity | assumption].
+  - auto_bind_comp.
+  - auto_bind_comp.
+Qed.
+
+#[export] Instance Bind_val : Bind val.
+Proof.
+  split; intros; [now apply vbind_id | now apply vbind_comp].
+Qed.
+#[export] Instance Bind_expr : Bind expr.
+Proof.
+  split; intros; [now apply ebind_id | now apply ebind_comp].
+Qed.
+#[export] Instance Bind_ectx : Bind ectx.
+Proof.
+  split; intros; [now apply kbind_id | now apply kbind_comp].
+Qed.
+
+(*** Operational semantics *)
+
+Record state := State {
+                   inputs : list nat;
+                   outputs : list nat;
+                 }.
+#[export] Instance state_inhabited : Inhabited state := populate (State [] []).
+
+Definition update_input (s : state) : nat * state :=
+  match s.(inputs) with
+  | [] => (0, s)
+  | n::ns =>
+      (n, {| inputs := ns; outputs := s.(outputs) |})
+  end.
+Definition update_output (n:nat) (s : state) : state :=
+  {| inputs := s.(inputs); outputs := n::s.(outputs) |}.
+
+
+Inductive head_step {S} : expr S → state → expr S → state → ectx S → nat * nat → Prop :=
+| BetaS e1 v2 σ K :
+  head_step (App (Val $ RecV e1) (Val v2)) σ (subst (Inc := inc) ((subst (Inc := inc) e1) (shift v2)) (RecV e1)) σ K (1,0)
+| InputS σ n σ' K :
+  update_input σ = (n, σ') →
+  head_step Input σ (Val (LitV n)) σ' K (1, 1)
+| OutputS σ n σ' K :
+  update_output n σ = σ' →
+  head_step (Output (Val (LitV n))) σ (Val (LitV 0)) σ' K (1, 1)
+| NatOpS op v1 v2 v3 σ K :
+  nat_op_interp op v1 v2 = Some v3 →
+  head_step (NatOp op (Val v1) (Val v2)) σ
+            (Val v3) σ K (0, 0)
+| IfTrueS n e1 e2 σ K :
+  n > 0 →
+  head_step (If (Val (LitV n)) e1 e2) σ
+            e1 σ K (0, 0)
+| IfFalseS n e1 e2 σ K :
+  n = 0 →
+  head_step (If (Val (LitV n)) e1 e2) σ
+    e2 σ K (0, 0)
+| CallccS e σ K :
+  head_step (Callcc e) σ (subst (Inc := inc) e (ContV K)) σ K (0, 0)
+.
+
+Lemma head_step_io_01 {S} (e1 e2 : expr S) σ1 σ2 K n m :
+  head_step e1 σ1 e2 σ2 K (n,m) → m = 0 ∨ m = 1.
+Proof.  inversion 1; eauto. Qed.
+Lemma head_step_unfold_01 {S} (e1 e2 : expr S) σ1 σ2 K n m :
+  head_step e1 σ1 e2 σ2 K (n,m) → n = 0 ∨ n = 1.
+Proof.  inversion 1; eauto. Qed.
+Lemma head_step_no_io {S} (e1 e2 : expr S) σ1 σ2 K n :
+  head_step e1 σ1 e2 σ2 K (n,0) → σ1 = σ2.
+Proof.  inversion 1; eauto. Qed.
+
+(** Carbonara from heap lang *)
+Global Instance fill_item_inj {S} (Ki : ectx S) : Inj (=) (=) (fill Ki).
+Proof. induction Ki; intros ???; simplify_eq/=; auto with f_equal. Qed.
+
+Lemma fill_item_val {S} Ki (e : expr S) :
+  is_Some (to_val (fill Ki e)) → is_Some (to_val e).
+Proof. intros [v ?]. induction Ki; simplify_option_eq; eauto. Qed.
+
+Lemma val_head_stuck {S} (e1 : expr S) σ1 e2 σ2 K m : head_step e1 σ1 e2 σ2 K m → to_val e1 = None.
+Proof. destruct 1; naive_solver. Qed.
+
+Fixpoint ectx_compose {S} (K1 K2 : ectx S) : ectx S
+  := match K1 with
+     | EmptyK => K2
+     | OutputK K => OutputK (ectx_compose K K2)
+     | IfK K e₁ e₂ => IfK (ectx_compose K K2) e₁ e₂
+     | AppLK e K => AppLK e (ectx_compose K K2)
+     | AppRK K v => AppRK (ectx_compose K K2) v
+     | NatOpLK op e K => NatOpLK op e (ectx_compose K K2)
+     | NatOpRK op K v => NatOpRK op (ectx_compose K K2) v
+     | ThrowLK K e => ThrowLK (ectx_compose K K2) e
+     | ThrowRK v K => ThrowRK v (ectx_compose K K2)
+     end.
+
+Lemma fill_app {S} (K1 K2 : ectx S) e : fill (ectx_compose K1 K2) e = fill K1 (fill K2 e).
+Proof.
+  revert K2.
+  revert e.
+  induction K1 as [| ?? IH
+                  | ?? IH
+                  | ??? IH
+                  | ?? IH
+                  | ???? IH
+                  | ??? IH
+                  | ?? IH
+                  | ??? IH];
+    simpl; first done; intros e' K2; rewrite IH; reflexivity.
+Qed.
+
+Lemma fill_val : ∀ {S} K (e : expr S), is_Some (to_val (fill K e)) → is_Some (to_val e).
+Proof.
+  intros S K.
+  induction K as [| ?? IH
+                 | ?? IH
+                 | ??? IH
+                 | ?? IH
+                 | ???? IH
+                 | ??? IH
+                 | ?? IH
+                 | ??? IH]=> e' //=;
+                              inversion 1 as [? HH]; inversion HH.
+Qed.
+
+Lemma fill_not_val : ∀ {S} K (e : expr S), to_val e = None → to_val (fill K e) = None.
+Proof.
+  intros S K e. rewrite !eq_None_not_Some.
+  eauto using fill_val.
+Qed.
+
+Lemma fill_empty {S} (e : expr S) : fill EmptyK e = e.
+Proof. reflexivity. Qed.
+Lemma fill_comp {S} K1 K2 (e : expr S) : fill K2 (fill K1 e) = fill (ectx_compose K2 K1) e.
+Proof. by rewrite fill_app. Qed.
+Global Instance fill_inj {S} (K : ectx S) : Inj (=) (=) (fill K).
+Proof.
+  induction K as [| ?? IH
+                 | ?? IH
+                 | ??? IH
+                 | ?? IH
+                 | ???? IH
+                 | ??? IH
+                 | ?? IH
+                 | ??? IH];
+    rewrite /Inj; naive_solver.
+Qed.
+
+Inductive prim_step {S} : ∀ (e1 : expr S) (σ1 : state)
+          (e2 : expr S) (σ2 : state) (n : nat * nat), Prop :=
+| Ectx_step e1 σ1 e2 σ2 n (K : ectx S) e1' e2' :
+  e1 = fill K e1' → e2 = fill K e2' →
+  head_step e1' σ1 e2' σ2 K n → prim_step e1 σ1 e2 σ2 n
+| Throw_step e1 σ e2 (K : ectx S) v K' :
+  e1 = (fill K (Throw (of_val v) (ContV K'))) ->
+  e2 = (fill K' v) ->
+  prim_step e1 σ e2 σ (0, 0).
+
+Lemma prim_step_pure {S} (e1 e2 : expr S) σ1 σ2 n :
+  prim_step e1 σ1 e2 σ2 (n,0) → σ1 = σ2.
+Proof.
+  inversion 1; simplify_eq/=.
+  - inversion H2; eauto.
+  - reflexivity.
+Qed.
+
+Inductive prim_steps {S} : expr S → state → expr S → state → nat * nat → Prop :=
+| prim_steps_zero e σ :
+  prim_steps e σ e σ (0, 0)
+| prim_steps_abit e1 σ1 e2 σ2 e3 σ3 n1 m1 n2 m2 :
+  prim_step e1 σ1 e2 σ2 (n1, m1) →
+  prim_steps e2 σ2 e3 σ3 (n2, m2) →
+  prim_steps e1 σ1 e3 σ3 (plus n1 n2, plus m1 m2)
+.
+
+Lemma Ectx_step' {S} (K : ectx S) e1 σ1 e2 σ2 efs :
+  head_step e1 σ1 e2 σ2 K efs → prim_step (fill K e1) σ1 (fill K e2) σ2 efs.
+Proof. econstructor; eauto. Qed.
+
+Lemma prim_steps_app {S} nm1 nm2 (e1 e2 e3 : expr S) σ1 σ2 σ3 :
+  prim_steps e1 σ1 e2 σ2 nm1 → prim_steps e2 σ2 e3 σ3 nm2 →
+  prim_steps e1 σ1 e3 σ3 (plus nm1.1 nm2.1, plus nm1.2 nm2.2).
+Proof.
+  intros Hst. revert nm2.
+  induction Hst; intros [n' m']; simplify_eq/=; first done.
+  rewrite -!Nat.add_assoc. intros Hsts.
+  econstructor; eauto.
+  by apply (IHHst (n',m')).
+Qed.
+
+Lemma prim_step_steps {S} nm (e1 e2 : expr S) σ1 σ2 :
+  prim_step e1 σ1 e2 σ2 nm → prim_steps e1 σ1 e2 σ2 nm.
+Proof.
+  destruct nm as [n m]. intro Hs.
+  rewrite -(Nat.add_0_r n).
+  rewrite -(Nat.add_0_r m).
+  econstructor; eauto.
+  by constructor.
+Qed.
+
+(*** Type system *)
+
+Inductive ty :=
+  | Tnat : ty | Tarr : ty → ty → ty | Tcont : ty → ty.
+
+Inductive typed {S : Set} (Γ : S -> ty) : expr S → ty → Prop :=
+| typed_Val (τ : ty) (v : val S)  :
+  typed_val Γ v τ →
+  typed Γ (Val v) τ
+| typed_App (τ1 τ2 : ty) e1 e2 :
+  typed Γ e1 (Tarr τ1 τ2) →
+  typed Γ e2 τ1 →
+  typed Γ (App e1 e2) τ2
+| typed_NatOp e1 e2 op :
+  typed Γ e1 Tnat →
+  typed Γ e2 Tnat →
+  typed Γ (NatOp op e1 e2) Tnat
+| typed_If e0 e1 e2 τ :
+  typed Γ e0 Tnat →
+  typed Γ e1 τ →
+  typed Γ e2 τ →
+  typed Γ (If e0 e1 e2) τ
+| typed_Input :
+  typed Γ Input Tnat
+| typed_Output e :
+  typed Γ e Tnat →
+  typed Γ (Output e) Tnat
+| typed_Throw e1 e2 τ τ' :
+  typed Γ e1 τ ->
+  typed Γ e2 (Tcont τ) ->
+  typed Γ (Throw e1 e2) τ'
+| typed_Callcc e τ :
+  typed (Γ ▹ Tcont τ) e τ ->
+  typed Γ (Callcc e) τ
+with typed_val {S : Set} (Γ : S -> ty) : val S → ty → Prop :=
+| typed_Var (τ : ty) (v : S)  :
+  Γ v = τ →
+  typed_val Γ (VarV v) τ
+| typed_Lit n :
+  typed_val Γ (LitV n) Tnat
+| typed_RecV (τ1 τ2 : ty) (e : expr (inc (inc S))) :
+  typed (Γ ▹ (Tarr τ1 τ2) ▹ τ1) e τ2 →
+  typed_val Γ (RecV e) (Tarr τ1 τ2)
+.
