theories/input_lang_callcc/logpred.v
@@ -1,0 +1,299 @@
+(** Unary (Kripke) logical relation for the IO lang *)
+From Equations Require Import Equations.
+From gitrees Require Import gitree program_logic.
+From gitrees.input_lang Require Import lang interp.
+
+Section io_lang.
+  Context {sz : nat}.
+  Variable rs : gReifiers sz.
+  Context `{!subReifier reify_io rs}.
+  Notation F := (gReifiers_ops rs).
+  Context {R} `{!Cofe R}.
+  Context `{!SubOfe natO R}.
+  Notation IT := (IT F R).
+  Notation ITV := (ITV F R).
+  Context `{!invGS Σ, !stateG rs R Σ, !na_invG Σ}.
+  Notation iProp := (iProp Σ).
+
+  Variable s : stuckness.
+  Context {A:ofe}.
+  Variable (P : A → iProp).
+  Context `{!NonExpansive P}.
+
+  Local Notation tyctx := (tyctx ty).
+  Local Notation expr_pred := (expr_pred s rs P).
+
+  Program Definition interp_tnat : ITV -n> iProp := λne αv,
+    (∃ n : nat, αv ≡ RetV n)%I.
+  Solve All Obligations with solve_proper.
+  Program Definition interp_tarr (Φ1 Φ2 : ITV -n> iProp) := λne αv,
+    (□ ∀ σ βv, has_substate σ -∗
+               Φ1 βv -∗
+               expr_pred (IT_of_V αv ⊙ (IT_of_V βv)) (λne v, ∃ σ', Φ2 v ∗ has_substate σ'))%I.
+  Solve All Obligations with solve_proper.
+
+  Fixpoint interp_ty (τ : ty) : ITV -n> iProp :=
+    match τ with
+    | Tnat => interp_tnat
+    | Tarr τ1 τ2 => interp_tarr (interp_ty τ1) (interp_ty τ2)
+    end.
+
+  Definition ssubst_valid {S} (Γ : tyctx S) ss := ssubst_valid rs interp_ty Γ ss.
+
+  #[global] Instance io_lang_interp_ty_pers  τ βv : Persistent (io_lang.interp_ty τ βv).
+  Proof. induction τ; apply _. Qed.
+  #[global] Instance ssubst_valid_pers {S} (Γ : tyctx S) ss : Persistent (ssubst_valid  Γ  ss).
+  Proof. apply _. Qed.
+
+  Program Definition valid1 {S}  (Γ : tyctx S) (α : interp_scope S -n> IT) (τ : ty) : iProp :=
+    (∀ σ ss, has_substate σ -∗ ssubst_valid Γ ss -∗
+          expr_pred (α (interp_ssubst ss)) (λne v, ∃ σ', interp_ty τ v ∗ has_substate σ'))%I.
+  Solve Obligations with solve_proper.
+
+  Lemma compat_nat {S} n (Ω : tyctx S) :
+    ⊢ valid1 Ω (interp_nat rs n) Tnat.
+  Proof.
+    iIntros (σ αs) "Hs Has".
+    simpl. iApply expr_pred_ret. simpl.
+    eauto with iFrame.
+  Qed.
+  Lemma compat_var {S} Ω τ (v : var S) :
+    typed_var Ω v τ →
+    ⊢ valid1 Ω (interp_var v) τ.
+  Proof.
+    intros Hv.
+    iIntros (σ ss) "Hs Has". simpl.
+    unfold ssubst_valid.
+    iInduction Hv as [|? ? ? Ω v] "IH" forall (ss); simpl.
+    - dependent elimination ss as [cons_ssubst αv ss].
+      rewrite ssubst_valid_cons.
+      simp interp_var. simpl.
+      iDestruct "Has" as "[H _]".
+      iApply expr_pred_ret; simpl; eauto with iFrame.
+    - dependent elimination ss as [cons_ssubst αv ss].
+      rewrite ssubst_valid_cons.
+      simp interp_var. simpl.
+      iDestruct "Has" as "[_ H]".
+      by iApply ("IH" with "Hs H").
+  Qed.
+  Lemma compat_if {S} (Γ : tyctx S) τ α β1 β2 :
+    ⊢ valid1 Γ α Tnat -∗
+      valid1 Γ β1 τ -∗
+      valid1 Γ β2 τ -∗
+      valid1 Γ (interp_if rs α β1 β2) τ.
+  Proof.
+    iIntros "H0 H1 H2".
+    iIntros (σ ss) "Hs #Has".
+    iSpecialize ("H0" with "Hs Has").
+    simpl. iApply (expr_pred_bind (IFSCtx _ _) with "H0").
+    iIntros (αv) "Ha/=".
+    iDestruct "Ha" as (σ') "[Ha Hs]".
+    iDestruct "Ha" as (n) "Hn".
+    unfold IFSCtx. iIntros (x) "Hx".
+    iRewrite "Hn".
+    destruct n as [|n].
+    - rewrite IF_False; last lia.
+      iApply ("H2" with "Hs Has Hx").
+    - rewrite IF_True; last lia.
+      iApply ("H1" with "Hs Has Hx").
+  Qed.
+  Lemma compat_input {S} (Γ : tyctx S) :
+    ⊢ valid1 Γ (interp_input rs) Tnat.
+  Proof.
+    iIntros (σ ss) "Hs #Has".
+    iApply expr_pred_frame.
+    destruct (update_input σ) as [n σ'] eqn:Hinp.
+    iApply (wp_input with "Hs") .
+    { eauto. }
+    iNext. iIntros "_ Hs".
+    iApply wp_val. simpl. eauto with iFrame.
+  Qed.
+  Lemma compat_output {S} (Γ : tyctx S) α :
+    ⊢ valid1 Γ α Tnat → valid1 Γ (interp_output rs α) Tnat.
+  Proof.
+    iIntros "H".
+    iIntros (σ ss) "Hs #Has".
+    iSpecialize ("H" with "Hs Has").
+    simpl.
+    iApply (expr_pred_bind (get_ret _) with "H").
+    iIntros (αv) "Ha".
+    iDestruct "Ha" as (σ') "[Ha Hs]".
+    iDestruct "Ha" as (n) "Hn".
+    iApply expr_pred_frame.
+    iRewrite "Hn".
+    rewrite get_ret_ret.
+    iApply (wp_output with "Hs").
+    { reflexivity. }
+    iNext. iIntros "_ Hs /=".
+    eauto with iFrame.
+  Qed.
+  Lemma compat_app {S} (Γ : tyctx S) α β τ1 τ2 :
+    ⊢ valid1 Γ α (Tarr τ1 τ2) -∗
+      valid1 Γ β τ1 -∗
+      valid1 Γ (interp_app rs α β) τ2.
+  Proof.
+    iIntros "H1 H2".
+    iIntros (σ ss) "Hs #Has". simpl.
+    iSpecialize ("H2" with "Hs Has").
+    iApply (expr_pred_bind (AppRSCtx _) with "H2").
+    iIntros (βv) "Hb/=".
+    iDestruct "Hb" as (σ') "[Hb Hs]".
+    unfold AppRSCtx.
+    iSpecialize ("H1" with "Hs Has").
+    iApply (expr_pred_bind (AppLSCtx (IT_of_V βv)) with "H1").
+    iIntros (αv) "Ha".
+    iDestruct "Ha" as (σ'') "[Ha Hs]".
+    unfold AppLSCtx.
+    iApply ("Ha" with "Hs Hb").
+  Qed.
+
+  Lemma compat_rec {S} (Γ : tyctx S) τ1 τ2 α :
+    ⊢ □ valid1 (consC (Tarr τ1 τ2) (consC τ1 Γ)) α τ2 -∗
+      valid1 Γ (interp_rec rs α) (Tarr τ1 τ2).
+  Proof.
+    iIntros "#H". iIntros (σ ss) "Hs #Hss".
+    pose (env := (interp_ssubst ss)). fold env.
+    simp subst_expr.
+    pose (f := (ir_unf rs α env)).
+    iAssert (interp_rec rs α env ≡ IT_of_V $ FunV (Next f))%I as "Hf".
+    { iPureIntro. apply interp_rec_unfold. }
+    iRewrite "Hf". iApply expr_pred_ret. simpl.
+    iExists _. iFrame. iModIntro.
+    iLöb as "IH". iSimpl.
+    clear σ.
+    iIntros (σ βv) "Hs #Hw".
+    iIntros (x) "Hx".
+    iApply wp_lam.
+    iNext.
+    pose (ss' := cons_ssubst (FunV (Next f)) (cons_ssubst βv ss)).
+    iSpecialize ("H" $! _ ss' with "Hs []").
+    { unfold ssubst_valid.
+      unfold ss'.
+      rewrite !ssubst_valid_cons.
+      by iFrame "IH Hw Hss". }
+    unfold f. simpl.
+    unfold ss'. simp interp_ssubst.
+    iAssert (IT_of_V (FunV (Next f)) ≡ interp_rec rs α env)%I as "Heq".
+    { rewrite interp_rec_unfold. done. }
+    iRewrite -"Heq". by iApply "H".
+  Qed.
+
+  Lemma compat_natop  {S} (Γ : tyctx S) op α β :
+    ⊢ valid1 Γ α Tnat -∗
+      valid1 Γ β Tnat -∗
+      valid1 Γ (interp_natop _ op α β) Tnat.
+  Proof.
+    iIntros "H1 H2".
+    iIntros (σ ss) "Hs #Has". simpl.
+    iSpecialize ("H2" with "Hs Has").
+    iApply (expr_pred_bind (NatOpRSCtx _ _) with "H2").
+    iIntros (βv) "Hb/=".
+    iDestruct "Hb" as (σ') "[Hb Hs]".
+    unfold NatOpRSCtx.
+    iSpecialize ("H1" with "Hs Has").
+    iApply (expr_pred_bind (NatOpLSCtx _ (IT_of_V βv)) with "H1").
+    iIntros (αv) "Ha".
+    iDestruct "Ha" as (σ'') "[Ha Hs]".
+    unfold NatOpLSCtx.
+    iDestruct "Hb" as (n1) "Hb".
+    iDestruct "Ha" as (n2) "Ha".
+    iRewrite "Hb". iRewrite "Ha".
+    simpl. iApply expr_pred_frame.
+    rewrite NATOP_Ret. iApply wp_val. simpl.
+    eauto with iFrame.
+  Qed.
+
+  Lemma fundamental {S} (Γ : tyctx S) e τ :
+    typed Γ e τ → ⊢ valid1 Γ (interp_expr rs e) τ
+  with fundamental_val {S} (Γ : tyctx S) v τ :
+    typed_val Γ v τ → ⊢ valid1 Γ (interp_val rs v) τ.
+  Proof.
+    - destruct 1.
+      + by iApply fundamental_val.
+      + by iApply compat_var.
+      + iApply compat_rec; iApply fundamental; eauto.
+      + iApply compat_app; iApply fundamental; eauto.
+      + iApply compat_natop; iApply fundamental; eauto.
+      + iApply compat_if;  iApply fundamental; eauto.
+      + iApply compat_input.
+      + iApply compat_output; iApply fundamental; eauto.
+    - destruct 1.
+      + iApply compat_nat.
+      + iApply compat_rec; iApply fundamental; eauto.
+  Qed.
+  Lemma fundmanetal_closed (e : expr []) (τ : ty) :
+    typed empC e τ →
+    ⊢ valid1 empC (interp_expr rs e) τ.
+  Proof. apply fundamental. Qed.
+
+End io_lang.
+
+Arguments interp_ty {_ _ _ _ _ _ _ _ _ _ _ _} τ.
+Arguments interp_tarr {_ _ _ _ _ _ _ _ _ _ _} Φ1 Φ2.
+
+Local Definition rs : gReifiers _ := gReifiers_cons reify_io gReifiers_nil.
+
+Variable Hdisj : ∀ (Σ : gFunctors) (P Q : iProp Σ), disjunction_property P Q.
+
+Lemma logpred_adequacy cr Σ R `{!Cofe R, SubOfe natO R}`{!invGpreS Σ}`{!statePreG rs R Σ} τ (α : unitO -n> IT (gReifiers_ops rs) R) (β : IT (gReifiers_ops rs) R) st st' k :
+  (∀ `{H1 : !invGS Σ} `{H2: !stateG rs R Σ},
+      (£ cr ⊢ valid1 rs notStuck (λ _:unitO, True)%I empC α τ)%I) →
+  ssteps (gReifiers_sReifier rs) (α ()) st β st' k →
+  (∃ β1 st1, sstep (gReifiers_sReifier rs) β st' β1 st1)
+   ∨ (∃ βv, IT_of_V βv ≡ β).
+Proof.
+  intros Hlog Hst.
+  destruct (IT_to_V β) as [βv|] eqn:Hb.
+  { right. exists βv. apply IT_of_to_V'. rewrite Hb; eauto. }
+  left.
+  cut ((∃ β1 st1, sstep (gReifiers_sReifier rs) β st' β1 st1)
+      ∨ (∃ e, β ≡ Err e ∧ notStuck e)).
+  { intros [?|He]; first done.
+    destruct He as [? [? []]]. }
+  eapply (wp_safety cr); eauto.
+  { apply Hdisj. }
+  { by rewrite Hb. }
+  intros H1 H2.
+  exists (interp_ty (s:=notStuck) (P:=(λ _:unitO, True)) τ)%I. split.
+  { apply _. }
+  iIntros "[Hcr  Hst]".
+  iPoseProof (Hlog with "Hcr") as "Hlog".
+  destruct st as [σ []].
+  iAssert (has_substate σ) with "[Hst]" as "Hs".
+  { unfold has_substate, has_full_state.
+    assert (of_state rs (IT (gReifiers_ops rs) _) (σ,()) ≡
+            of_idx rs (IT (gReifiers_ops rs) _) sR_idx (sR_state σ)) as ->; last done.
+    intro j. unfold sR_idx. simpl.
+    unfold of_state, of_idx.
+    destruct decide as [Heq|]; last first.
+    { inv_fin j; first done.
+      intros i. inversion i. }
+    inv_fin j; last done.
+    intros Heq.
+    rewrite (eq_pi _ _ Heq eq_refl)//.
+  }
+  iSpecialize ("Hlog" $! σ with "Hs []").
+  { iApply ssubst_valid_nil. }
+  iSpecialize ("Hlog" $! tt with "[//]").
+  iApply (wp_wand with"Hlog").
+  iIntros ( βv). simpl. iDestruct 1 as (_) "[H _]".
+  iDestruct "H" as (σ1') "[$ Hsts]".
+  done.
+Qed.
+
+Lemma io_lang_safety e τ σ st' (β : IT (sReifier_ops (gReifiers_sReifier rs)) natO) k :
+  typed empC e τ →
+  ssteps (gReifiers_sReifier rs) (interp_expr _ e ()) (σ,()) β st' k →
+  (∃ β1 st1, sstep (gReifiers_sReifier rs) β st' β1 st1)
+   ∨ (∃ βv, IT_of_V βv ≡ β).
+Proof.
+  intros Htyped Hsteps.
+  pose (Σ:=#[invΣ;stateΣ rs natO]).
+  assert (invGpreS Σ).
+  { apply _. }
+  assert (statePreG rs natO Σ).
+  { apply _. }
+  eapply (logpred_adequacy 0 Σ); eauto.
+  intros ? ?. iIntros "_".
+  by iApply fundamental.
+Qed.
